# 848. Shifting Letters
Difficulty medium

You are given a string s of lowercase English letters and an integer array shifts of the same length.

Call the shift() of a letter, the next letter in the alphabet, (wrapping around so that 'z' becomes 'a').

For example, shift('a') = 'b', shift('t') = 'u', and shift('z') = 'a'.
Now for each shifts[i] = x, we want to shift the first i + 1 letters of s, x times.

Return the final string after all such shifts to s are applied.


## Example 1:
```
Input: s = "abc", shifts = [3,5,9]
Output: "rpl"
Explanation: We start with "abc".
After shifting the first 1 letters of s by 3, we have "dbc".
After shifting the first 2 letters of s by 5, we have "igc".
After shifting the first 3 letters of s by 9, we have "rpl", the answer.
```


## Example 2:
```
Input: s = "aaa", shifts = [1,2,3]
Output: "gfd"
```


```
Constraints:

1 <= s.length <= 105
s consists of lowercase English letters.
shifts.length == s.length
0 <= shifts[i] <= 109
```


#
```
class Solution {
public:
    string shiftingLetters(string s, vector<int>& shifts) {
        // Presum begin
        // int n = shifts.size();
        // vector<int> suf(n);
        // suf[n - 1] = shifts[n - 1];
        // for (int i = n - 2; i >= 0; --i) suf[i] = (suf[i + 1] + shifts[i]) % 26;
        // for (int i = 0; i < s.length(); ++i) s[i] = (((s[i] - 'a' + suf[i]) % 26) + 'a');
        // return s;
        // Presum end


        // Backward iterate begin
        int sum = 0;
        for (int i = s.length() - 1; i >= 0; --i) {
            sum = (sum + shifts[i]) % 26;
            s[i] = ((s[i] - 'a' + sum) % 26) + 'a';
        }
        return s;
        // Backward iterate end
    }
};
```